outputs/vTaskSwitchContext.v
@@ -37,41 +37,40 @@ Definition CLZ (n : N) : N := clz(n) 32.
 (* Postcondition *)
 Definition time_of_vTaskSwitchContext (t : trace)
     (mem : addr -> N)
-    (reg_init_sp_22241_32 : N)	(* sp *)
-    (reg_init_gp_22242_32 : N)	(* gp *)
+    (gp : N)
   : Prop :=
     cycle_count_of_trace t =
 (* 0x8000137c *)   time_mem
-                   + (if mem Ⓓ[reg_init_gp_22242_32 + 0xfffff860] =? 0x0
+                   + (if mem Ⓓ[gp + 0xfffff860] =? 0x0
                      then
                        time_branch + 
 (* 0x80001390 *)       2 + time_mem + time_mem + time_mem + 2 + time_mem + time_mem + 2 + time_mem
-                       + (if negb(mem Ⓓ[mem Ⓓ[mem Ⓓ[reg_init_gp_22242_32 + 0xfffff898] + 0x30]] =? 0xa5a5a5a5)
+                       + (if negb(mem Ⓓ[mem Ⓓ[mem Ⓓ[gp + 0xfffff898] + 0x30]] =? 0xa5a5a5a5)
                          then
                            time_branch + 
 (* 0x800013d0 *)           time_inf
                          else
                            3 + 
 (* 0x800013b8 *)           time_mem
-                           + (if negb(mem Ⓓ[mem Ⓓ[mem Ⓓ[reg_init_gp_22242_32 + 0xfffff898] + 0x30] + 0x4] =? mem Ⓓ[mem Ⓓ[mem Ⓓ[reg_init_gp_22242_32 + 0xfffff898] + 0x30]])
+                           + (if negb(mem Ⓓ[mem Ⓓ[mem Ⓓ[gp + 0xfffff898] + 0x30] + 0x4] =? mem Ⓓ[mem Ⓓ[mem Ⓓ[gp + 0xfffff898] + 0x30]])
                              then
                                time_branch + 
 (* 0x800013d0 *)               time_inf
                              else
                                3 + 
 (* 0x800013c0 *)               time_mem
-                               + (if negb(mem Ⓓ[mem Ⓓ[mem Ⓓ[reg_init_gp_22242_32 + 0xfffff898] + 0x30] + 0x8] =? mem Ⓓ[mem Ⓓ[mem Ⓓ[reg_init_gp_22242_32 + 0xfffff898] + 0x30] + 0x4])
+                               + (if negb(mem Ⓓ[mem Ⓓ[mem Ⓓ[gp + 0xfffff898] + 0x30] + 0x8] =? mem Ⓓ[mem Ⓓ[mem Ⓓ[gp + 0xfffff898] + 0x30] + 0x4])
                                  then
                                    time_branch + 
 (* 0x800013d0 *)                   time_inf
                                  else
                                    3 + 
 (* 0x800013c8 *)                   time_mem
-                                   + (if mem Ⓓ[mem Ⓓ[mem Ⓓ[reg_init_gp_22242_32 + 0xfffff898] + 0x30] + 0xc] =? mem Ⓓ[mem Ⓓ[mem Ⓓ[reg_init_gp_22242_32 + 0xfffff898] + 0x30] + 0x8]
+                                   + (if mem Ⓓ[mem Ⓓ[mem Ⓓ[gp + 0xfffff898] + 0x30] + 0xc] =? mem Ⓓ[mem Ⓓ[mem Ⓓ[gp + 0xfffff898] + 0x30] + 0x8]
                                      then
                                        time_branch + 
-(* 0x800013e0 *)                       time_mem + 2 + (3 + clz (mem Ⓓ[reg_init_gp_22242_32 + 0xfffff880]) 32) + 2 + 2 + 36 + 2 + 2 + 2 + time_mem + 2 + 2 + time_mem + time_mem
-                                       + (if negb(mem Ⓓ[mem Ⓓ[reg_init_gp_22242_32 + 0xffffffec * CLZ(mem Ⓓ[reg_init_gp_22242_32 + 0xfffff880]) + 0xfffffed4] + 0x4] =? 0xfffffed8 + 0xffffffec * CLZ(mem Ⓓ[reg_init_gp_22242_32 + 0xfffff880]) + reg_init_gp_22242_32)
+(* 0x800013e0 *)                       time_mem + 2 + (3 + clz (mem Ⓓ[gp + 0xfffff880]) 32) + 2 + 2 + 36 + 2 + 2 + 2 + time_mem + 2 + 2 + time_mem + time_mem
+                                       + (if negb(mem Ⓓ[mem Ⓓ[gp + 0xffffffec * CLZ(mem Ⓓ[gp + 0xfffff880]) + 0xfffffed4] + 0x4] =? 0xfffffed8 + 0xffffffec * CLZ(mem Ⓓ[gp + 0xfffff880]) + gp)
                                          then
                                            time_branch + 
 (* 0x80001424 *)                           2 + 36 + time_mem + 2 + time_mem + time_mem + time_mem + time_mem + time_mem + 2 + time_branch
@@ -96,47 +95,43 @@ Definition time_of_vTaskSwitchContext (t : trace)
 (* Memory Regions *)
 Definition memory_regions
     (mem : addr -> N)
-    (reg_init_sp_22241_32 : N)	(* sp *)
-    (reg_init_gp_22242_32 : N)	(* gp *)
+    (gp : N)
     := map (fun x => (4, x)) [
-		reg_init_gp_22242_32 + 0xffffffec * CLZ(mem Ⓓ[reg_init_gp_22242_32 + 0xfffff880]) + 0xfffffed4;
-		mem Ⓓ[mem Ⓓ[reg_init_gp_22242_32 + 0xfffff898] + 0x30];
-		reg_init_sp_22241_32 + 0xfffffff8;
-		reg_init_sp_22241_32 + 0xfffffffc;
-		mem Ⓓ[mem Ⓓ[reg_init_gp_22242_32 + 0xfffff898] + 0x30] + 0x8;
-		mem Ⓓ[reg_init_gp_22242_32 + 0xffffffec * CLZ(mem Ⓓ[reg_init_gp_22242_32 + 0xfffff880]) + 0xfffffed4] + 0x4;
-		reg_init_gp_22242_32 + 0xffffffec * CLZ(mem Ⓓ[reg_init_gp_22242_32 + 0xfffff880]) + 0xfffffedc;
-		mem Ⓓ[reg_init_gp_22242_32 + 0xffffffec * CLZ(mem Ⓓ[reg_init_gp_22242_32 + 0xfffff880]) + 0xfffffed4] + 0xc;
-		mem Ⓓ[reg_init_gp_22242_32 + 0xfffff898] + 0x30;
-		reg_init_gp_22242_32 + 0xfffff860;
-		mem Ⓓ[mem Ⓓ[reg_init_gp_22242_32 + 0xfffff898] + 0x30] + 0xc;
-		reg_init_gp_22242_32 + 0xfffff880;
-		reg_init_gp_22242_32 + 0xfffff898;
-		reg_init_gp_22242_32 + 0xfffff874;
-		mem Ⓓ[mem Ⓓ[reg_init_gp_22242_32 + 0xfffff898] + 0x30] + 0x4
+		0x7ffffffb;
+		mem Ⓓ[mem Ⓓ[gp + 0xfffff898] + 0x30];
+		0x7ffffff7;
+		gp + 0xfffff880;
+		mem Ⓓ[gp + 0xffffffec * CLZ(mem Ⓓ[gp + 0xfffff880]) + 0xfffffed4] + 0xc;
+		gp + 0xffffffec * CLZ(mem Ⓓ[gp + 0xfffff880]) + 0xfffffedc;
+		mem Ⓓ[mem Ⓓ[gp + 0xfffff898] + 0x30] + 0x8;
+		mem Ⓓ[gp + 0xffffffec * CLZ(mem Ⓓ[gp + 0xfffff880]) + 0xfffffed4] + 0x4;
+		gp + 0xfffff874;
+		gp + 0xffffffec * CLZ(mem Ⓓ[gp + 0xfffff880]) + 0xfffffed4;
+		mem Ⓓ[mem Ⓓ[gp + 0xfffff898] + 0x30] + 0xc;
+		mem Ⓓ[gp + 0xfffff898] + 0x30;
+		gp + 0xfffff898;
+		mem Ⓓ[mem Ⓓ[gp + 0xfffff898] + 0x30] + 0x4;
+		gp + 0xfffff860
       ].
 
 Definition noverlaps
     (mem : addr -> N)
-    (reg_init_sp_22241_32 : N)	(* sp *)
-    (reg_init_gp_22242_32 : N)	(* gp *)
-    :=  create_noverlaps (memory_regions mem reg_init_sp_22241_32 reg_init_gp_22242_32).
+    (gp : N)
+    :=  create_noverlaps (memory_regions mem gp).
 
 
 (* Invariants *)
 Definition vTaskSwitchContext_timing_invs 
     (mem : addr -> N)
-    (reg_init_sp_22241_32 : N)	(* sp *)
-    (reg_init_gp_22242_32 : N)	(* gp *)
+    (gp : N)
     (t : trace) : option Prop :=
 match t with (Addr a, s) :: t' => match a with
-| 0x8000137c => Some (s R_SP = Ⓓreg_init_sp_22241_32 /\
-			s R_GP = Ⓓreg_init_gp_22242_32 /\
+| 0x8000137c => Some (s R_GP = Ⓓgp /\
 			s V_MEM32 = Ⓜmem /\
-			noverlaps mem reg_init_sp_22241_32 reg_init_gp_22242_32 /\
+			noverlaps mem gp /\
 			cycle_count_of_trace t' = 0)
 | 0x80001424 => Some (exists mem, s V_MEM32 = Ⓜmem /\
-			noverlaps mem reg_init_sp_22241_32 reg_init_gp_22242_32 /\
+			noverlaps mem gp /\
 			cycle_count_of_trace t' =   
   (* 0x8000137c *)   time_mem + 
                        time_branch + 
@@ -148,8 +143,8 @@ match t with (Addr a, s) :: t' => match a with
                        3 + 
   (* 0x800013c8 *)   time_mem + 
                        time_branch + 
-  (* 0x800013e0 *)   time_mem + 2 + (3 + clz (mem Ⓓ[reg_init_gp_22242_32 + 0xfffff880]) 32) + 2 + 2 + 36 + 2 + 2 + 2 + time_mem + 2 + 2 + time_mem + time_mem
-                     + (if negb(mem Ⓓ[mem Ⓓ[reg_init_gp_22242_32 + 0xffffffec * CLZ(mem Ⓓ[reg_init_gp_22242_32 + 0xfffff880]) + 0xfffffed4] + 0x4] =? 0xfffffed8 + 0xffffffec * CLZ(mem Ⓓ[reg_init_gp_22242_32 + 0xfffff880]) + reg_init_gp_22242_32)
+  (* 0x800013e0 *)   time_mem + 2 + (3 + clz (mem Ⓓ[gp + 0xfffff880]) 32) + 2 + 2 + 36 + 2 + 2 + 2 + time_mem + 2 + 2 + time_mem + time_mem
+                     + (if negb(mem Ⓓ[mem Ⓓ[gp + 0xffffffec * CLZ(mem Ⓓ[gp + 0xfffff880]) + 0xfffffed4] + 0x4] =? 0xfffffed8 + 0xffffffec * CLZ(mem Ⓓ[gp + 0xfffff880]) + gp)
                        then
                          time_branch + 0
                        else
@@ -158,7 +153,7 @@ match t with (Addr a, s) :: t' => match a with
                        )
 		)
 | 0x8000138c | 0x8000144c => Some (exists mem, s V_MEM32 = Ⓜmem /\
-			time_of_vTaskSwitchContext t mem reg_init_sp_22241_32 reg_init_gp_22242_32)
+			time_of_vTaskSwitchContext t mem gp)
 | _ => None end | _ => None end
 .
 
@@ -170,16 +165,15 @@ Definition lifted_vTaskSwitchContext : program :=
 
 (* Proof *)
 Theorem vTaskSwitchContext_timing:
-  forall s t s' x' mem sp gp
+  forall s t s' x' mem gp
     (ENTRY: startof t (x',s') = (Addr entry_addr, s))
     (MDL: models rvtypctx s)
-    (NVL: create_noverlaps (memory_regions mem sp gp))
+    (NVL: create_noverlaps (memory_regions mem gp))
     (MEM: s V_MEM32 = Ⓜmem)
-    (SP: s R_SP = Ⓓsp)
     (GP: s R_GP = Ⓓgp),
   satisfies_all
     lifted_vTaskSwitchContext
-    (vTaskSwitchContext_timing_invs mem sp gp)
+    (vTaskSwitchContext_timing_invs mem gp)
     exits
  ((x',s')::t).
 Proof using.
